[CDCL+MR] more proofs; start new rule;

Weidenbach_Book/CDCL/Pragmatic_CDCL_MR.thy
@@ -5,7 +5,6 @@ begin
 fun to_mr_state :: \<open>'v prag_st \<times> 'v stackWit \<Rightarrow> 'v clauses \<times> 'v clauses \<times> 'v stackWit \<times> 'v set\<close> where
   \<open>to_mr_state ((M, N, U, D, NE, UE, NS, US, N0, U0), S) = (N + NE + NS + N0, U + UE + US + U0, S, atms_of_mm (N + NE + NS + N0 + U + UE + US + U0) \<union> atms_of_ms (wit_clause ` set S))\<close>
 
-  
 lemma cdcl_backtrack_rules:
   assumes \<open>cdcl_backtrack V W\<close> and \<open>pcdcl_all_struct_invs V\<close>
   shows \<open>rules (to_mr_state (V, S)) (to_mr_state (W, S))\<close>
@@ -70,6 +69,84 @@ lemma pcdcl_core_rules:
     using cdcl_backtrack_rules[of V W S] by auto
   done
 
+lemma cdcl_resolution_rules: 
+  assumes \<open>cdcl_resolution V W\<close>
+    \<open>pcdcl_all_struct_invs V\<close>
+  shows \<open>rules\<^sup>*\<^sup>* (to_mr_state (V, S)) (to_mr_state (W, S))\<close>
+  using assms
+proof (cases rule: cdcl_resolution.cases)
+  case (resolution_LL M C C' N U L D NE UE NS US N0 U0) note V = this(1) and W = this(2) and _ = this(3)
+  then have \<open>insert (add_mset L C)
+   (insert (add_mset (- L) C')
+     (set_mset N \<union> set_mset NE \<union> set_mset NS \<union> set_mset N0 \<union>
+      (set_mset U \<union> set_mset UE \<union> set_mset US \<union> set_mset U0))) \<Turnstile>p
+    C' + C\<close>
+    using true_clss_cls_or_true_clss_cls_or_not_true_clss_cls_or[of \<open>set_mset (pget_all_init_clss V + pget_all_learned_clss V)\<close> L C' C]
+    by auto
+  then have R: \<open>rules (pget_all_init_clss V, pget_all_learned_clss V, S, {} \<union> atms_of (remdups_mset (C + C')) \<union> atms_of_mm (pget_all_init_clss V) \<union>
+    atms_of_mm (pget_all_learned_clss V) \<union>
+    atms_of_mm (wit_clause `# mset S))
+    (pget_all_init_clss V, add_mset (remdups_mset (C + C')) (pget_all_learned_clss V), S, {} \<union> atms_of (remdups_mset (C + C')) \<union> atms_of_mm (pget_all_init_clss V) \<union>
+    atms_of_mm (pget_all_learned_clss V) \<union>
+    atms_of_mm (wit_clause `# mset S))\<close>
+    using learn_minus[of \<open>pget_all_init_clss V\<close> \<open>pget_all_learned_clss V\<close> \<open>remdups_mset (C+C')\<close> S \<open>{}\<close>]
+    by (auto simp: V W ac_simps)
+  have \<open>rules (to_mr_state (V, S)) (to_mr_state (W, S))\<close>
+    apply (rule arg_cong2[where f = rules, THEN iffD2, OF _ _ R])
+    subgoal by (auto simp: V)
+    subgoal by (auto simp: W V)
+    done
+  then show ?thesis by blast
+next
+  case (resolution_II M N L C C' U D NE UE NS US N0 U0) note V = this(1) and W = this(2) and _ = this(3)
+  then have \<open>insert (add_mset L C)
+   (insert (add_mset (- L) C')
+     (set_mset N \<union> set_mset NE \<union> set_mset NS \<union> set_mset N0 \<union>
+      (set_mset U \<union> set_mset UE \<union> set_mset US \<union> set_mset U0))) \<Turnstile>p
+    C' + C\<close>
+    using true_clss_cls_or_true_clss_cls_or_not_true_clss_cls_or[of \<open>set_mset (pget_all_init_clss V + pget_all_learned_clss V)\<close> L C' C]
+    by auto
+  then have R: \<open>rules (to_mr_state (V, S))
+    (pget_all_init_clss V, add_mset (remdups_mset (C + C')) (pget_all_learned_clss V), S, {} \<union> atms_of (remdups_mset (C + C')) \<union> atms_of_mm (pget_all_init_clss V) \<union>
+    atms_of_mm (pget_all_learned_clss V) \<union>
+    atms_of_mm (wit_clause `# mset S))\<close> (is \<open>rules ?A ?B\<close>)
+    using learn_minus[of \<open>pget_all_init_clss V\<close> \<open>pget_all_learned_clss V\<close> \<open>remdups_mset (C+C')\<close> S \<open>{}\<close>]
+    by (auto simp: V W ac_simps)
+  moreover have R: \<open>rules ?B
+    ( add_mset (remdups_mset (C + C')) (pget_all_init_clss V),(pget_all_learned_clss V), S, {} \<union> atms_of (remdups_mset (C + C')) \<union> atms_of_mm (pget_all_init_clss V) \<union>
+    atms_of_mm (pget_all_learned_clss V) \<union>
+    atms_of_mm (wit_clause `# mset S))\<close> (is \<open>rules _ ?C\<close>)
+    using strenghten[of \<open>pget_all_init_clss V\<close>  \<open>remdups_mset (C+C')\<close>  \<open>pget_all_learned_clss V\<close> S \<open>{}\<close>]
+    by (auto simp: V W ac_simps)
+  moreover have \<open> ?C = (to_mr_state (W, S))\<close>
+    by (auto simp: V W ac_simps)
+  ultimately show \<open>rules\<^sup>*\<^sup>* (to_mr_state (V, S)) (to_mr_state (W, S))\<close>
+    by auto
+next
+  case (resolution_IL M C C' N L U D NE UE NS US N0 U0) note V = this(1) and W = this(2) and _ = this(3)
+  then have \<open>insert (add_mset (-L) C')
+   (insert (add_mset L C)
+     (set_mset N \<union> set_mset NE \<union> set_mset NS \<union> set_mset N0 \<union>
+      (set_mset U \<union> set_mset UE \<union> set_mset US \<union> set_mset U0))) \<Turnstile>p
+    C' + C\<close>
+    using true_clss_cls_or_true_clss_cls_or_not_true_clss_cls_or[of \<open>set_mset (pget_all_init_clss V + pget_all_learned_clss V)\<close> L C' C]
+    by auto
+  then have R: \<open>rules (pget_all_init_clss V, pget_all_learned_clss V, S, {} \<union> atms_of (remdups_mset (C + C')) \<union> atms_of_mm (pget_all_init_clss V) \<union>
+    atms_of_mm (pget_all_learned_clss V) \<union>
+    atms_of_mm (wit_clause `# mset S))
+    (pget_all_init_clss V, add_mset (remdups_mset (C + C')) (pget_all_learned_clss V), S, {} \<union> atms_of (remdups_mset (C + C')) \<union> atms_of_mm (pget_all_init_clss V) \<union>
+    atms_of_mm (pget_all_learned_clss V) \<union>
+    atms_of_mm (wit_clause `# mset S))\<close>
+    using learn_minus[of \<open>pget_all_init_clss V\<close> \<open>pget_all_learned_clss V\<close> \<open>remdups_mset (C+C')\<close> S \<open>{}\<close>]
+    by (auto simp: V W ac_simps)
+  have \<open>rules (to_mr_state (V, S)) (to_mr_state (W, S))\<close>
+    apply (rule arg_cong2[where f = rules, THEN iffD2, OF _ _ R])
+    subgoal by (auto simp: V)
+    subgoal by (auto simp: W V)
+    done
+  then show ?thesis by blast
+qed
+
 lemma pcdcl_rules:
   \<open>pcdcl V W \<Longrightarrow> pcdcl_all_struct_invs V \<Longrightarrow> rules\<^sup>*\<^sup>* (to_mr_state (V, S)) (to_mr_state (W, S))\<close>
   apply (cases rule: pcdcl.cases, assumption)
@@ -92,17 +169,36 @@ lemma pcdcl_rules:
       by (auto simp: pcdcl_all_struct_invs_def ac_simps pcdcl_all_struct_invs_def
         cdcl\<^sub>W_restart_mset.cdcl\<^sub>W_all_struct_inv_def cdcl\<^sub>W_restart_mset.clauses_def cdcl\<^sub>W_restart_mset.no_strange_atm_def)
     done
-  subgoal apply (auto simp: cdcl_resolution.simps)
-    sorry
+  subgoal by (rule cdcl_resolution_rules)
   subgoal by (auto simp: cdcl_subsumed.simps Un_left_commute add_mset_commute)
   subgoal by (auto simp: cdcl_flush_unit.simps)
   subgoal by (auto simp: cdcl_inp_propagate.simps)
   subgoal by (auto simp: cdcl_inp_conflict.simps)
   subgoal by (auto simp: cdcl_unitres_true.simps)
   subgoal by (auto simp: cdcl_promote_false.simps)
-
+(*does not hold without the Ns \<Turnstile> Us which we do not really want to add as assumptiom*)
     oops
 
+text \<open>
+This is an attempt to create a rule derived from our inprocessing rules back to our cdcl:
 
+  \<^item> \<^term>\<open>add_mset (add_mset (-L) C)\<close> is on purpose a tautology to make sure that we do not lose variables. Although
 
+\<close>
+inductive cdcl_weaken :: \<open>'v prag_st \<times> 'v stackWit  \<Rightarrow> 'v prag_st \<times> 'v stackWit \<Rightarrow> bool\<close> where
+weaken:
+  \<open>cdcl_weaken ((M, add_mset C N, U, None, NE, UE, NS, US, N0, U0), S)
+    ((M, N, U, None, add_mset (add_mset (-L) C) NE, UE, NS, US, N0, U0), S @ [Witness I C])\<close>
+  if
+    "I \<Turnstile> C"  and "redundancy N C I N" and "consistent_interp I " and
+    "atm_of ` I \<subseteq> atms_of_mm (N+NE+NS+N0) \<union> atms_of_mm (wit_clause `# mset S)" and
+    \<open>L \<in># C\<close>
+
+lemma
+  assumes \<open>cdcl_weaken (V, S) (W, T)\<close> \<open>pcdcl_all_struct_invs V\<close>
+  shows
+    \<open>pcdcl_all_struct_invs W\<close> and
+    \<open>rules\<^sup>*\<^sup>*  (to_mr_state (V, S)) (to_mr_state (W, T))\<close>
+oops
+(*this will get tricky here*)
 end
